Correctness of translated expressions.

DataflowSyntax.v
@@ -21,12 +21,18 @@ with lexp : Type :=
   | Ewhen : laexp -> ident -> bool -> lexp.
 (* External operators are missing *)
 
+Scheme laexp_mult := Induction for laexp Sort Prop
+with lexp_mult := Induction for lexp Sort Prop.
+
 (* TODO: caexp: would be nicer if it were a record *)
 Inductive caexp : Type :=
   | CAexp : clock -> cexp -> caexp
 with cexp : Type :=
   | Emerge : ident -> caexp -> caexp -> cexp (* currently only binary merge *)
   | Eexp : lexp -> cexp.
+
+Scheme caexp_mult := Induction for caexp Sort Prop
+with cexp_mult := Induction for cexp Sort Prop.
 
 (** ** Equations *)
 
@@ -58,6 +64,15 @@ with freevar_laexp' (lae : laexp) (fvs : PS.t) : PS.t :=
   match lae with
     | LAexp ck e => freevar_lexp' e fvs
   end.
+
+Fixpoint memory_eq (mems: PS.t) (eq: equation) : PS.t :=
+  match eq with
+  | EqFby x _ _ => PS.add x mems
+  | _ => mems
+  end.
+
+Definition memories (eqs: list equation) : PS.t :=
+  List.fold_left memory_eq eqs PS.empty.
 
 (** The map containing global definitions. *)
 Require Coq.FSets.FMapPositive.
